cwf/effpresheaf.v
@@ -1,0 +1,164 @@
+Set Universe Polymorphism.
+Set Polymorphic Inductive Cumulativity.
+Set Primitive Projections.
+
+Record sig (A : Type) (B : A -> Type) := pair {
+  fst : A;
+  snd : B fst;
+}.
+
+Arguments pair {_ _}.
+Arguments fst {_ _}.
+Arguments snd {_ _}.
+
+Axiom ℙ : Set.
+Axiom le0 : ℙ -> ℙ -> Set.
+
+Definition le (p q : ℙ) := forall r, le0 q r -> le0 p r.
+
+Notation "p ≤ q" := (le p q) (at level 70).
+Notation "α ∘ β" := (fun (r : ℙ) (γ : le0 _ r) => α r (β r γ)) (at level 50).
+Notation "!" := (fun (r : ℙ) (γ : le0 _ r) => γ).
+Notation "α · t" := (fun (q : ℙ) (β : q ≤ _) => t q (β ∘ α)) (at level 50).
+
+Record Ctx := {
+  ctx_typ : forall (p : ℙ), Type;
+}.
+
+Coercion ctx_typ : Ctx >-> Funclass.
+
+Record Sub (Γ Δ : Ctx) := {
+  sub_fun : forall p (γ : forall q (α : q ≤ p), Γ q), Δ p;
+}.
+
+Coercion sub_fun : Sub >-> Funclass.
+
+Record Typ (Γ : Ctx) := {
+  typ_typ : forall p (γ : forall q (α : q ≤ p), Γ q), Type;
+}.
+
+Coercion typ_typ : Typ >-> Funclass.
+
+Record Trm (Γ : Ctx) (A : Typ Γ) := {
+  trm_elt : forall p (γ : forall q (α : q ≤ p), Γ q), A p γ;
+}.
+
+Arguments trm_elt {_ _}.
+
+Definition typ_sub {Γ Δ} (A : Typ Δ) (σ : Sub Γ Δ) : Typ Γ.
+Proof.
+unshelve econstructor.
+unshelve refine (fun p δ => A p (fun q α => σ q (α · δ))).
+Defined.
+
+Definition trm_sub {Γ Δ} {A : Typ Δ} (t : Trm Δ A) (σ : Sub Γ Δ) : Trm Γ (typ_sub A σ).
+Proof.
+unshelve econstructor.
+simpl; refine (fun p γ => _).
+refine (t.(trm_elt) _ _).
+Defined.
+
+Definition idn (Γ : Ctx) : Sub Γ Γ := Build_Sub _ _ (fun p γ => γ p !).
+
+Definition cmp {Γ Δ Ξ : Ctx} (σ : Sub Γ Δ) (τ : Sub Δ Ξ) : Sub Γ Ξ.
+Proof.
+unshelve econstructor.
+refine (fun p γ => τ _ (fun q α => σ q (α · γ))).
+Defined.
+
+Lemma typ_sub_idn : forall Γ A, typ_sub A (idn Γ) = A.
+Proof.
+reflexivity.
+Defined.
+
+Lemma typ_sub_cmp : forall Γ Δ Ξ A σ τ, typ_sub A (@cmp Γ Δ Ξ σ τ) = typ_sub (typ_sub A τ) σ.
+Proof.
+reflexivity.
+Defined.
+
+Lemma trm_sub_idn : forall Γ (A : Typ Γ) (x : Trm Γ A), trm_sub x (idn Γ) = x.
+Proof.
+reflexivity.
+Qed.
+
+Lemma trm_sub_cmp : forall Γ Δ Ξ (A : Typ Ξ) (x : Trm Ξ A) (σ : Sub Γ Δ) (τ : Sub Δ Ξ),
+  trm_sub x (cmp σ τ) = trm_sub (trm_sub x τ) σ.
+Proof.
+reflexivity.
+Qed.
+
+Definition ext (Γ : Ctx) (A : Typ Γ) : Ctx.
+Proof.
+unshelve econstructor.
+unshelve refine (fun p => sig _ _).
++ refine (forall q (α : q ≤ p), Γ q).
++ refine (fun γ => A p γ).
+Defined.
+
+Definition wkn {Γ Δ} (A : Typ Γ) (σ : Sub Γ Δ) : Sub (ext Γ A) Δ.
+Proof.
+constructor.
+refine (fun p γ => σ _ (fun q α => fst (γ q α) q !)).
+Defined.
+
+Definition lft {Γ Δ} (A : Typ Δ) (σ : Sub Γ Δ) : Sub (ext Γ (typ_sub A σ)) (ext Δ A).
+Proof.
+constructor.
+unshelve refine (fun γ => pair (σ γ.(fst)) γ.(snd)).
+Defined.
+
+Definition rel0 {Γ : Ctx} {A : Typ Γ} : Trm (ext Γ A) (typ_sub A (wkn A (idn _))).
+Proof.
+unshelve econstructor.
++ refine (fun γ p => γ.(snd).(fst) p).
++ refine (fun γ => γ.(snd).(snd)).
+Defined.
+
+Definition cns {Γ Δ} {A : Typ Γ} (σ : Sub Δ Γ) (x : Trm Δ (typ_sub A σ)) : Sub Δ (ext Γ A).
+Proof.
+unshelve econstructor.
+unshelve refine (fun δ => pair (σ δ) (pair (x.(trm_elt) _) (x.(trm_rel) _))).
+Defined.
+
+Definition Π {Γ : Ctx} (A : Typ Γ) (B : Typ (ext Γ A)) : Typ Γ.
+Proof.
+unshelve econstructor.
++ refine (fun γ p => forall (x : forall p, A.(typ_elt) γ p) (xε : A.(typ_rel) γ x), B.(typ_elt) (pair γ (pair x xε)) p).
++ cbn.
+  unshelve refine (fun γ f => forall (x : forall p, A.(typ_elt) γ p) (xε : A.(typ_rel) γ x), B.(typ_rel) _ _).
+  - refine (pair γ (pair x xε)).
+  - refine (fun p => f p _ _).
+Defined.
+
+Definition lam {Γ : Ctx} {A : Typ Γ} {B : Typ (ext Γ A)} (t : Trm (ext Γ A) B) : Trm Γ (Π A B).
+Proof.
+unshelve econstructor.
++ refine (fun γ p x xε => t.(trm_elt) _ _).
++ refine (fun γ x xε => t.(trm_rel) _).
+Defined.
+
+Definition app {Γ : Ctx} {A : Typ Γ} {B : Typ (ext Γ A)} (t : Trm Γ (Π A B)) (u : Trm Γ A) :
+  Trm Γ (typ_sub B (cns (idn Γ) u)).
+Proof.
+unshelve econstructor.
++ refine (fun γ p => t.(trm_elt) _ _ _ _).
++ refine (fun γ => t.(trm_rel) _ _ _).
+Defined.
+
+Definition Arr {Γ : Ctx} (A B : Typ Γ) := Π A (typ_sub B (wkn _ (idn _))).
+
+Definition Squash {Γ : Ctx} (A : Typ Γ) : Typ Γ.
+Proof.
+unshelve econstructor.
++ refine (fun γ p => A.(typ_elt) γ p).
++ refine (fun γ _ => True).
+Defined.
+
+Lemma choice {Γ} {A : Typ Γ} {B : Typ (ext Γ A)} : Trm Γ (Arr (Π A (Squash B)) (Squash (Π A B))).
+Proof.
+unshelve econstructor; cbn.
++ refine (fun γ p f fε x xε => _).
+  apply f.
++ constructor.
+Defined.
+*)
