cwf/readerparam.v
@@ -1,0 +1,118 @@
+Set Universe Polymorphism.
+Set Polymorphic Inductive Cumulativity.
+Set Primitive Projections.
+
+Record sig (A : Type) (B : A -> Type) := pair {
+  fst : A;
+  snd : B fst;
+}.
+
+Arguments pair {_ _}.
+Arguments fst {_ _}.
+Arguments snd {_ _}.
+
+Axiom ℙ : Set.
+
+Definition Ctx@{i} := Type@{i}.
+
+Record Typ@{i j k} (Γ : Ctx@{i}) := {
+  typ_elt : forall γ : Γ, (ℙ -> Type@{j});
+  typ_rel : forall γ : Γ, (forall p, typ_elt γ p) -> Type@{k};
+}.
+
+Arguments typ_elt {_}.
+Arguments typ_rel {_}.
+
+Record Trm@{i j k} (Γ : Ctx@{i}) (A : Typ@{i j k} Γ) := {
+  trm_elt : forall (γ : Γ) p, A.(typ_elt) γ p;
+  trm_rel : forall (γ : Γ), A.(typ_rel) γ (trm_elt γ);
+}.
+
+Arguments trm_elt {_ _}.
+Arguments trm_rel {_ _}.
+
+Record Sub@{i j} (Γ : Ctx@{i}) (Δ : Ctx@{j}) := {
+  sub_sub : Γ -> Δ;
+}.
+
+Coercion sub_sub : Sub >-> Funclass.
+
+Definition typ_sub {Γ Δ} (A : Typ Δ) (σ : Sub Γ Δ) : Typ Γ :=
+  Build_Typ _ (fun γ p => A.(typ_elt) (σ γ) p) (fun γ => A.(typ_rel) (σ γ)).
+
+Definition trm_sub {Γ Δ} {A : Typ Δ} (t : Trm Δ A) (σ : Sub Γ Δ) : Trm Γ (typ_sub A σ) :=
+  Build_Trm Γ (typ_sub A σ) (fun γ p => t.(trm_elt) (σ γ) p) (fun γ => t.(trm_rel) (σ γ)).
+
+Definition idn (Γ : Ctx) : Sub Γ Γ := Build_Sub _ _ (fun γ => γ).
+
+Definition ext (Γ : Ctx) (A : Typ Γ) : Ctx.
+Proof.
+unshelve refine (sig Γ (fun γ => sig (forall p, A.(typ_elt) γ p) (A.(typ_rel) γ))).
+Defined.
+
+Definition wkn {Γ Δ} (A : Typ Γ) (σ : Sub Γ Δ) : Sub (ext Γ A) Δ.
+Proof.
+constructor.
+refine (fun γ => σ (@fst _ _ γ)).
+Defined.
+
+Definition lft {Γ Δ} (A : Typ Δ) (σ : Sub Γ Δ) : Sub (ext Γ (typ_sub A σ)) (ext Δ A).
+Proof.
+constructor.
+unshelve refine (fun γ => pair (σ γ.(fst)) γ.(snd)).
+Defined.
+
+Definition rel0 {Γ : Ctx} {A : Typ Γ} : Trm (ext Γ A) (typ_sub A (wkn A (idn _))).
+Proof.
+unshelve econstructor.
++ refine (fun γ p => γ.(snd).(fst) p).
++ refine (fun γ => γ.(snd).(snd)).
+Defined.
+
+Definition cns {Γ Δ} {A : Typ Γ} (σ : Sub Δ Γ) (x : Trm Δ (typ_sub A σ)) : Sub Δ (ext Γ A).
+Proof.
+unshelve econstructor.
+unshelve refine (fun δ => pair (σ δ) (pair (x.(trm_elt) _) (x.(trm_rel) _))).
+Defined.
+
+Definition Π {Γ : Ctx} (A : Typ Γ) (B : Typ (ext Γ A)) : Typ Γ.
+Proof.
+unshelve econstructor.
++ refine (fun γ p => forall (x : forall p, A.(typ_elt) γ p) (xε : A.(typ_rel) γ x), B.(typ_elt) (pair γ (pair x xε)) p).
++ cbn.
+  unshelve refine (fun γ f => forall (x : forall p, A.(typ_elt) γ p) (xε : A.(typ_rel) γ x), B.(typ_rel) _ _).
+  - refine (pair γ (pair x xε)).
+  - refine (fun p => f p _ _).
+Defined.
+
+Definition lam {Γ : Ctx} {A : Typ Γ} {B : Typ (ext Γ A)} (t : Trm (ext Γ A) B) : Trm Γ (Π A B).
+Proof.
+unshelve econstructor.
++ refine (fun γ p x xε => t.(trm_elt) _ _).
++ refine (fun γ x xε => t.(trm_rel) _).
+Defined.
+
+Definition app {Γ : Ctx} {A : Typ Γ} {B : Typ (ext Γ A)} (t : Trm Γ (Π A B)) (u : Trm Γ A) :
+  Trm Γ (typ_sub B (cns (idn Γ) u)).
+Proof.
+unshelve econstructor.
++ refine (fun γ p => t.(trm_elt) _ _ _ _).
++ refine (fun γ => t.(trm_rel) _ _ _).
+Defined.
+
+Definition Arr {Γ : Ctx} (A B : Typ Γ) := Π A (typ_sub B (wkn _ (idn _))).
+
+Definition Squash {Γ : Ctx} (A : Typ Γ) : Typ Γ.
+Proof.
+unshelve econstructor.
++ refine (fun γ p => A.(typ_elt) γ p).
++ refine (fun γ _ => True).
+Defined.
+
+Lemma choice {Γ} {A : Typ Γ} {B : Typ (ext Γ A)} : Trm Γ (Arr (Π A (Squash B)) (Squash (Π A B))).
+Proof.
+unshelve econstructor; cbn.
++ refine (fun γ p f fε x xε => _).
+  apply f.
++ constructor.
+Defined.
